WIP

src/Var2.v
@@ -1,50 +1,101 @@
-Require Import String Omega Morph.
+Require Import String Omega Morph Setoid Morphisms.
 Arguments string_dec !s1 !s2.
+
+(* Pointwise equality *)
+
+Notation "f =p= g" :=
+  (pointwise_relation _ eq f g)
+    (at level 70).
+
+Add Parametric Morphism {A B} : (@pointwise_relation A B eq)
+  with signature
+    (pointwise_relation A eq ==>
+       pointwise_relation A eq ==>
+         Basics.impl)
+    as pointwise_relation_index_mor.
+  unfold pointwise_relation; intros.
+  intro. intro.
+  rewrite <- H.
+  rewrite <- H0.
+  easy.
+Qed.
+
+(* Pointwise equality for nsets *)
+
+Notation "f =pn= g" :=
+  (forall_relation
+     (fun V => pointwise_relation (_ (_ + V)) eq) f g)
+    (at level 70).
 
 (* Name indices are [nat]s *)
 Definition index := nat.
 
-(* Functions from [index]s that we treat like streams *)
-Definition iindex A := index -> A.
+(* Liftable functions from [index]s to nsets that we treat
+   like streams *)
+Definition iindex (T : nset) M := forall V, index -> T (M + V).
 
-Definition get_idx {A} (i : index) (l : iindex A) := l i.
-Arguments get_idx {A} i l /.
+Definition get_idx {T M} (i : index) (f : iindex T M) :=
+  fun V => f V i.
+Arguments get_idx {T M} i f V /.
 
-Definition drop_idx {A} (i : index) (l : iindex A) : iindex A :=
-  fun (j : index) =>
-    if Compare_dec.le_lt_dec i j then get_idx (S j) l
-    else get_idx j l.
+Definition drop_idx {T M} (i : index) (f : iindex T M) :
+  iindex T M :=
+  fun V (j : index) =>
+    if Compare_dec.le_lt_dec i j then get_idx (S j) f V
+    else get_idx j f V.
 
-Definition insert_idx {A} (i : index) (a : A) (l : iindex A)
-  : iindex A :=
-  fun (j : index) =>
+Definition insert_idx {T : nset} {M} (i : index)
+           (a : forall V, T (M + V)) (f : iindex T M)
+  : iindex T M :=
+  fun V (j : index) =>
     match Compare_dec.lt_eq_lt_dec i j with
-    | inleft (left _) => get_idx (pred j) l
-    | inleft (right _) => a
-    | inright _ => get_idx j l
+    | inleft (left _) => get_idx (pred j) f V
+    | inleft (right _) => a V
+    | inright _ => get_idx j f V
     end.  
 
-(* Extensionality of these primitives *)
+(* Morphism definitions *)
 
-Lemma get_idx_ext {A} i (l1 : iindex A) l2 :
-  (forall j, l1 j = l2 j) ->
-  get_idx i l1 = get_idx i l2.
-Proof. intro Heq; cbn; easy. Qed.
+Add Parametric Morphism {T : nset} {M} i : (@get_idx T M i)
+    with signature
+      (forall_relation
+         (fun V => pointwise_relation index (@eq (T (M + V))))
+         ==> forall_relation (fun V => @eq (T (M + V))))
+    as get_idx_mor.
+  intros * Heq *; intro V. cbn.
+  rewrite Heq; easy.
+Qed.
 
-Lemma drop_idx_ext {A} i (l1 : iindex A) l2 j :
-  (forall j, l1 j = l2 j) ->
-  drop_idx i l1 j = drop_idx i l2 j.
-Proof.
-  intro Heq; unfold drop_idx; cbn.
+Add Parametric Morphism {A} i : (@drop_idx A i)
+    with signature
+      (pointwise_relation index eq ==>
+          pointwise_relation index eq)
+    as drop_idx_mor.
+  intros * Heq; intro; unfold drop_idx; cbn.
   rewrite Heq, Heq; easy.
 Qed.
 
-Lemma insert_idx_ext {A} i a (l1 : iindex A) l2 j :
-  (forall j, l1 j = l2 j) ->
-  insert_idx i a l1 j = insert_idx i a l2 j.
-Proof.
-  intro Heq; unfold insert_idx; cbn.
+Add Parametric Morphism {A} i : (@drop_idx A i)
+    with signature
+      (pointwise_relation index eq ==> eq ==> eq)
+    as drop_idx_mor_eta.
+  apply drop_idx_mor.
+Qed.
+
+Add Parametric Morphism {A} i a : (@insert_idx A i a)
+    with signature
+      (pointwise_relation index eq ==>
+          pointwise_relation index eq)
+    as insert_idx_mor.
+  intros * Heq; intro; unfold insert_idx; cbn.
   rewrite Heq, Heq; easy.
+Qed.
+
+Add Parametric Morphism {A} i a : (@insert_idx A i a)
+    with signature
+      (pointwise_relation index eq ==> eq ==> eq)
+    as insert_idx_mor_eta.
+  apply insert_idx_mor.
 Qed.
 
 (* Useful [iindex index]s *)
@@ -61,54 +112,54 @@ Definition unshift_idx (i : index) :=
 
 (* Reductions *)
 
-Lemma rw_drop_idx_ge {A} i (l : iindex A) j :
+Lemma rw_drop_idx_ge {A} i (f : iindex A) j :
   i <= j ->
-  drop_idx i l j = l (S j).
+  drop_idx i f j = f (S j).
 Proof.
   intros; unfold drop_idx.
   destruct (le_lt_dec i j); try easy; omega.
 Qed.
 
-Lemma rw_drop_idx_lt {A} i (l : iindex A) j :
+Lemma rw_drop_idx_lt {A} i (f : iindex A) j :
   S j <= i ->
-  drop_idx i l j = l j.
+  drop_idx i f j = f j.
 Proof.
   intros; unfold drop_idx.
   destruct (le_lt_dec i j); try easy; omega.
 Qed.
 
-Lemma rw_drop_idx_same {A} i (l : iindex A) :
-  drop_idx i l i = l (S i).
+Lemma rw_drop_idx_same {A} i (f : iindex A) :
+  drop_idx i f i = f (S i).
 Proof.
   apply rw_drop_idx_ge; auto.
 Qed.
 
-Lemma rw_insert_idx_gt {A} i a (l : iindex A) j :
+Lemma rw_insert_idx_gt {A} i a (f : iindex A) j :
   S i <= j ->
-  insert_idx i a l j = l (pred j).
+  insert_idx i a f j = f (pred j).
 Proof.
   intros; unfold insert_idx.
   destruct (lt_eq_lt_dec i j) as [[|]|]; try easy; omega.
 Qed.
 
-Lemma rw_insert_idx_eq {A} i a (l : iindex A) j :
+Lemma rw_insert_idx_eq {A} i a (f : iindex A) j :
   i = j ->
-  insert_idx i a l j = a.
+  insert_idx i a f j = a.
 Proof.
   intros; unfold insert_idx.
   destruct (lt_eq_lt_dec i j) as [[|]|]; try easy; omega.
 Qed.
 
-Lemma rw_insert_idx_lt {A} i a (l : iindex A) j :
+Lemma rw_insert_idx_lt {A} i a (f : iindex A) j :
   S j <= i ->
-  insert_idx i a l j = l j.
+  insert_idx i a f j = f j.
 Proof.
   intros; unfold insert_idx.
   destruct (lt_eq_lt_dec i j) as [[|]|]; try easy; omega.
 Qed.
 
-Lemma rw_insert_idx_same {A} i a (l : iindex A) :
-  insert_idx i a l i = a.
+Lemma rw_insert_idx_same {A} i a (f : iindex A) :
+  insert_idx i a f i = a.
 Proof.
   apply rw_insert_idx_eq; auto.
 Qed.
@@ -184,21 +235,23 @@ Ltac case_order i j :=
 
 (* Beta and eta rules for [iindex] operations *)
 
-Lemma iindex_beta_get {A} i (a : A) l :
-  get_idx i (insert_idx i a l) = a.
+Lemma iindex_beta_get {A} i (a : A) f :
+  get_idx i (insert_idx i a f) = a.
 Proof.
   cbn; autorewrite with rw_idxs; easy.
 Qed.
 
-Lemma iindex_beta_drop {A} i (a : A) l j :
-  drop_idx i (insert_idx i a l) j = l j.
+Lemma iindex_beta_drop {A} i (a : A) f :
+  drop_idx i (insert_idx i a f) =p= f.
 Proof.
+  intro j.
   case_order i j; easy.
 Qed.
 
-Lemma iindex_eta {A} i (l : iindex A) j :
-  insert_idx i (get_idx i l) (drop_idx i l) j = l j.
+Lemma iindex_eta {A} i (f : iindex A) :
+  insert_idx i (get_idx i f) (drop_idx i f) =p= f.
 Proof.
+  intro j.
   case_order i j; f_equal; omega.
 Qed.
 
@@ -207,102 +260,53 @@ Hint Rewrite @iindex_beta_get @iindex_beta_drop @iindex_eta
 
 (* Commuting [iindex] operations *)
 
-Lemma swap_drop_idx_drop_idx {A} i j (l : iindex A) k :
-  drop_idx i (drop_idx j l) k
-  = drop_idx (unshift_idx i j)
-      (drop_idx (shift_idx j i) l) k.
+Lemma swap_drop_idx_drop_idx {A} i j (f : iindex A) :
+  drop_idx i (drop_idx j f)
+  =p= drop_idx (unshift_idx i j)
+        (drop_idx (shift_idx j i) f).
 Proof.
+  intro k.
   case_order i j;
     case_order j k; try easy;
       case_order i k; try easy;
         case_order j (S k); easy.
 Qed.
 
-Lemma swap_insert_idx_insert_idx {A} i a j b (l : iindex A) k :
-  insert_idx i a (insert_idx j b l) k
-  = insert_idx (shift_idx i j) b
-      (insert_idx (unshift_idx j i) a l) k.
+Lemma swap_insert_idx_insert_idx {A} i a j b (f : iindex A) :
+  insert_idx i a (insert_idx j b f)
+  =p= insert_idx (shift_idx i j) b
+      (insert_idx (unshift_idx j i) a f).
 Proof.
+  intro k.
   case_order i j;
     case_order j k; try easy;
       case_order i k; try easy;
         case_order j (pred k); easy.
 Qed.
 
-Lemma swap_drop_idx_insert_idx {A} i j a (l : iindex A) k :
+Lemma swap_drop_idx_insert_idx {A} i j a (f : iindex A) :
   i <> j ->
-  drop_idx i (insert_idx j a l) k
-  = insert_idx (unshift_idx i j) a
-      (drop_idx (unshift_idx j i) l) k.
+  drop_idx i (insert_idx j a f)
+  =p= insert_idx (unshift_idx i j) a
+        (drop_idx (unshift_idx j i) f).
 Proof.
-  intro Hneq.
+  intros Hneq k.
   case_order i j; try contradiction;
     case_order i k; try easy;
       case_order j k; try easy;
         case_order j (S k); easy.     
 Qed.
 
-Lemma swap_insert_idx_drop_idx {A} i j a (l : iindex A) k :
-  insert_idx i a (drop_idx j l) k
-  = drop_idx (shift_idx i j)
-      (insert_idx (shift_idx (shift_idx i j) i) a l) k.
+Lemma swap_insert_idx_drop_idx {A} i j a (f : iindex A) :
+  insert_idx i a (drop_idx j f)
+  =p= drop_idx (shift_idx i j)
+      (insert_idx (shift_idx (shift_idx i j) i) a f).
 Proof.
+  intro k.
   case_order i j;
     case_order i k; try easy;
       case_order j k; try easy.
 Qed.
-
-(* Pre-composition of [iindex index] values *)
-
-Definition compose_idx {A} (l1 : iindex index) (l2 : iindex A) :=
-  fun (i : index) => get_idx (get_idx i l1) l2.
-
-Lemma compose_idx_assoc {A} l1 l2 (l3 : iindex A) i :
-  compose_idx (compose_idx l1 l2) l3 i
-  = compose_idx l1 (compose_idx l2 l3) i.
-Proof.
-  unfold compose_idx; cbn; easy.
-Qed.
-
-Lemma compose_idx_id {A} (l : iindex A) i :
-  compose_idx id_idx l i = l i.
-Proof.
-  unfold compose_idx; cbn; easy.
-Qed.
-
-Lemma compose_idx_drop {A} i l1 (l2 : iindex A) j :
-  compose_idx (drop_idx i l1) l2 j
-  = drop_idx i (compose_idx l1 l2) j.
-Proof.
-  unfold compose_idx; case_order i j; easy.
-Qed.
-
-Lemma compose_idx_shift {A} i (l : iindex A) j :
-  compose_idx (shift_idx i) l j
-  = drop_idx i l j.
-Proof.
-  unfold shift_idx; rewrite compose_idx_drop.
-  apply drop_idx_ext; intro; rewrite compose_idx_id; easy.
-Qed.
-
-Lemma compose_idx_insert {A} i j l1 (l2 : iindex A) k :
-  compose_idx (insert_idx i j l1) l2 k
-  = insert_idx i (get_idx j l2) (compose_idx l1 l2) k.
-Proof.
-  unfold compose_idx; case_order i k; easy.
-Qed.
-
-Lemma compose_idx_unshift {A} i (l : iindex A) j :
-  compose_idx (unshift_idx i) l j
-  = insert_idx i (get_idx i l) l j.
-Proof.
-  unfold unshift_idx; rewrite compose_idx_insert.
-  apply insert_idx_ext; intro; rewrite compose_idx_id; easy.
-Qed.
-
-Hint Rewrite @compose_idx_assoc @compose_idx_id @compose_idx_drop
-     @compose_idx_shift @compose_idx_insert @compose_idx_unshift
-  : rw_idxs.
 
 (* Free names are a pair of a string and an index *)
 
@@ -315,92 +319,115 @@ Definition name_of_string s := mkname s 0.
 Coercion name_of_string : string >-> name.
 Bind Scope string_scope with name.
 
+(* Useful lemma *)
+Lemma name_neq_string_eq_index_neq n m :
+  n <> m -> n_string n = n_string m -> n_index n <> n_index m.
+Proof.
+  intros Hneq Heq1 Heq2; apply Hneq.
+  replace n with (mkname (n_string n) (n_index n)) by easy.
+  replace (n_string n) with (n_string m) by easy.
+  replace (n_index n) with (n_index m) by easy.
+  easy.
+Qed.
+
 (* Functions from [names]s that we treat like direct
    sums of streams *)
 Definition iname A := name -> A.
 
-Definition project_name {A} s (l : iname A) : iindex A :=
-  fun (i : index) => l (mkname s i).
-Arguments project_name {A} s l i /.
+Definition project_name {A} s (f : iname A) : iindex A :=
+  fun (i : index) => f (mkname s i).
+Arguments project_name {A} s f i /.
 
-Definition with_name {A} s (li : iindex A) (ln : iname A)
+Definition with_name {A} s (f : iindex A) (g : iname A)
   : iname A :=
   fun (n : name) =>
-    if string_dec (n_string n) s then get_idx (n_index n) li
-    else ln n.
+    if string_dec (n_string n) s then get_idx (n_index n) f
+    else g n.
 
-Definition get_name {A} (n : name) (l : iname A) :=
-  get_idx (n_index n) (project_name (n_string n) l).
+Definition get_name {A} (n : name) (f : iname A) :=
+  get_idx (n_index n) (project_name (n_string n) f).
 
-Definition drop_name {A} (n : name) (l : iname A) : iname A :=
+Definition drop_name {A} (n : name) (f : iname A) : iname A :=
   with_name (n_string n)
-    (drop_idx (n_index n) (project_name (n_string n) l)) l.
+    (drop_idx (n_index n) (project_name (n_string n) f)) f.
 
-Definition insert_name {A} (n : name) (a : A) (l : iname A)
+Definition insert_name {A} (n : name) (a : A) (f : iname A)
   : iname A :=
   with_name (n_string n)
-    (insert_idx (n_index n) a (project_name (n_string n) l)) l.
+    (insert_idx (n_index n) a (project_name (n_string n) f)) f.
 
-(* Extensionality of these primitives *)
+(* Morphism definitions *)
 
-Lemma project_name_ext {A} s (l1 : iname A) l2 n :
-  (forall m, l1 m = l2 m) ->
-  project_name s l1 n = project_name s l2 n.
-Proof. intro Heq; cbn; easy. Qed.
+Add Parametric Morphism {A} s : (@project_name A s)
+    with signature
+      (pointwise_relation name eq ==>
+         pointwise_relation index eq)
+    as project_name_mor.
+  intros; unfold project_name; easy.
+Qed.
 
-Lemma with_name_ext1 {A} s (li1 : iindex A) li2 ln n :
-  (forall i, li1 i = li2 i) ->
-  with_name s li1 ln n = with_name s li2 ln n.
-Proof.
-  intro Heq; unfold with_name; cbn.
+Add Parametric Morphism {A} s : (@project_name A s)
+    with signature
+      (pointwise_relation name eq ==> eq ==> eq)
+    as project_name_mor_eta.
+  apply project_name_mor.
+Qed.
+
+Add Parametric Morphism {A} s : (@with_name A s)
+    with signature
+      (pointwise_relation index eq ==>
+         pointwise_relation name eq ==>
+           pointwise_relation name eq)
+    as with_name_mor.
+  intros * Heq1 * Heq2; unfold with_name; cbn.
+  intro; rewrite Heq1, Heq2; easy.
+Qed.
+
+Add Parametric Morphism {A} s : (@with_name A s)
+    with signature
+      (pointwise_relation index eq ==>
+         pointwise_relation name eq ==> eq ==> eq)
+    as with_name_mor_eta.
+  apply with_name_mor.
+Qed.
+
+Add Parametric Morphism {A} n : (@get_name A n)
+    with signature
+      (pointwise_relation name eq ==> eq)
+    as get_name_mor.
+  intros; unfold get_name; cbn; easy.
+Qed.
+
+Add Parametric Morphism {A} n : (@drop_name A n)
+    with signature
+      (pointwise_relation name eq ==>
+          pointwise_relation name eq)
+    as drop_name_mor.
+  intros * Heq; intro; unfold drop_name; cbn.
   rewrite Heq; easy.
 Qed.
 
-Lemma with_name_ext2 {A} s (li : iindex A) ln1 ln2 n :
-  (forall m, ln1 m = ln2 m) ->
-  with_name s li ln1 n = with_name s li ln2 n.
-Proof.
-  intro Heq; unfold with_name; cbn.
+Add Parametric Morphism {A} i : (@drop_name A i)
+    with signature
+      (pointwise_relation name eq ==> eq ==> eq)
+    as drop_name_mor_eta.
+  apply drop_name_mor.
+Qed.
+
+Add Parametric Morphism {A} n a : (@insert_name A n a)
+    with signature
+      (pointwise_relation name eq ==>
+          pointwise_relation name eq)
+    as insert_name_mor.
+  intros * Heq; intro; unfold insert_name; cbn.
   rewrite Heq; easy.
 Qed.
 
-Lemma with_name_ext {A} s (li1 : iindex A) li2 ln1 ln2 n :
-  (forall i, li1 i = li2 i) ->
-  (forall m, ln1 m = ln2 m) ->
-  with_name s li1 ln1 n = with_name s li2 ln2 n.
-Proof.
-  intros Heq1 Heq2.
-  erewrite with_name_ext1 by exact Heq1.
-  apply with_name_ext2; easy.
-Qed.
-
-Lemma get_name_ext {A} n (l1 : iname A) l2 :
-  (forall m, l1 m = l2 m) ->
-  get_name n l1 = get_name n l2.
-Proof.
-  intro Heq; unfold get_name.
-  apply get_idx_ext; intro.
-  apply project_name_ext; easy.
-Qed.
-
-Lemma drop_name_ext {A} n (l1 : iname A) l2 m :
-  (forall o, l1 o = l2 o) ->
-  drop_name n l1 m = drop_name n l2 m.
-Proof.
-  intro Heq; unfold drop_name.
-  apply with_name_ext; try easy; intro.
-  apply drop_idx_ext; intro.
-  apply project_name_ext; easy.
-Qed.
-
-Lemma insert_name_ext {A} n a (l1 : iname A) l2 m :
-  (forall o, l1 o = l2 o) ->
-  insert_name n a l1 m = insert_name n a l2 m.
-Proof.
-  intro Heq; unfold insert_name.
-  apply with_name_ext; try easy; intro.
-  apply insert_idx_ext; intro.
-  apply project_name_ext; easy.
+Add Parametric Morphism {A} i a : (@insert_name A i a)
+    with signature
+      (pointwise_relation name eq ==> eq ==> eq)
+    as insert_name_mor_eta.
+  apply insert_name_mor.
 Qed.
 
 (* Useful [iname name]s *)
@@ -417,81 +444,81 @@ Definition unshift_name (n : name) :=
 
 (* Reductions *)
 
-Lemma rw_with_name_eq {A} s li (ln : iname A) n :
+Lemma rw_with_name_eq {A} s f (g : iname A) n :
   s = n_string n ->
-  with_name s li ln n = li (n_index n).
+  with_name s f g n = f (n_index n).
 Proof.
   intro Heq; subst; unfold with_name.
   destruct (string_dec (n_string n) (n_string n));
     try contradiction; easy.
 Qed.
 
-Lemma rw_with_name_neq {A} s li (ln : iname A) n :
+Lemma rw_with_name_neq {A} s f (g : iname A) n :
   s <> n_string n ->
-  with_name s li ln n = ln n.
+  with_name s f g n = g n.
 Proof.
   intro Heq; unfold with_name.
   destruct (string_dec (n_string n) s); subst;
     try contradiction; easy.
 Qed.
 
-Lemma rw_with_name_same {A} li (ln : iname A) n :
-  with_name (n_string n) li ln n = li (n_index n).
+Lemma rw_with_name_same {A} f (g : iname A) n :
+  with_name (n_string n) f g n = f (n_index n).
 Proof.
   apply rw_with_name_eq; easy.
 Qed.
 
-Lemma rw_get_name {A} n (l : iname A) :
-  get_name n l = l n.
+Lemma rw_get_name {A} n (f : iname A) :
+  get_name n f = f n.
 Proof.
   unfold get_name; easy.
 Qed.
 
-Lemma rw_drop_name_indistinct {A} n (l : iname A) m :
+Lemma rw_drop_name_indistinct {A} n (f : iname A) m :
   n_string n = n_string m ->
-  drop_name n l m
-  = drop_idx (n_index n) (project_name (n_string n) l) (n_index m).
+  drop_name n f m
+  = drop_idx (n_index n) (project_name (n_string n) f) (n_index m).
 Proof.
   intro Heq; unfold drop_name.
   rewrite rw_with_name_eq; easy.
 Qed.
 
-Lemma rw_drop_name_distinct {A} n (l : iname A) m :
+Lemma rw_drop_name_distinct {A} n (f : iname A) m :
   n_string n <> n_string m ->
-  drop_name n l m = l m.
+  drop_name n f m = f m.
 Proof.
   intro Heq; unfold drop_name.
   rewrite rw_with_name_neq; easy.
 Qed.
 
-Lemma rw_drop_name_same {A} n (l : iname A) :
-  drop_name n l n
-  = l (mkname (n_string n) (S (n_index n))).
+Lemma rw_drop_name_same {A} n (f : iname A) :
+  drop_name n f n
+  = f (mkname (n_string n) (S (n_index n))).
 Proof.
   rewrite rw_drop_name_indistinct by easy.
   rewrite rw_drop_idx_same; easy.
 Qed.
 
-Lemma rw_insert_name_indistinct {A} n a (l : iname A) m :
+Lemma rw_insert_name_indistinct {A} n a (f : iname A) m :
   n_string n = n_string m ->
-  insert_name n a l m
+  insert_name n a f m
   = insert_idx (n_index n) a
-      (project_name (n_string n) l) (n_index m).
+      (project_name (n_string n) f) (n_index m).
 Proof.
   intro Heq; unfold insert_name.
   rewrite rw_with_name_eq; easy.
 Qed.
 
-Lemma rw_insert_name_distinct {A} n a (l : iname A) m :
+Lemma rw_insert_name_distinct {A} n a (f : iname A) m :
   n_string n <> n_string m ->
-  insert_name n a l m = l m.
+  insert_name n a f m = f m.
 Proof.
   intro Heq; unfold insert_name.
   rewrite rw_with_name_neq; easy.
 Qed.
 
-Lemma rw_insert_name_same {A} n a (l : iname A) :
-  insert_name n a l n = a.
+Lemma rw_insert_name_same {A} n a (f : iname A) :
+  insert_name n a f n = a.
 Proof.
   rewrite rw_insert_name_indistinct by easy.
   rewrite rw_insert_idx_same; easy.
@@ -570,30 +597,31 @@ Ltac case_string s1 s2 :=
 
 (* Beta and eta rules for [iname] operations *)
 
-Lemma iname_beta_project_same {A} s li (ln : iname A) i :
-  project_name s (with_name s li ln) i = li i.
+Lemma iname_beta_project_same {A} s f (g : iname A) :
+  project_name s (with_name s f g) =p= f.
 Proof.
-  cbn; autorewrite with rw_names; easy.
+  intro n; cbn; autorewrite with rw_names; easy.
 Qed.
 
-Lemma iname_beta_project_neq {A} s t li (ln : iname A) i :
+Lemma iname_beta_project_neq {A} s t f (g : iname A) :
   s <> t ->
-  project_name s (with_name t li ln) i = project_name s ln i.
+  project_name s (with_name t f g) =p= project_name s g.
 Proof.
-  intro; cbn.
-  autorewrite with rw_names; easy.
+  intros; intro; cbn; autorewrite with rw_names; easy.
 Qed.
 
-Lemma iname_beta_with_same {A} s li lj (ln : iname A) n :
-  with_name s li (with_name s lj ln) n
-  = with_name s li ln n.
+Lemma iname_beta_with_same {A} s f g (h : iname A) :
+  with_name s f (with_name s g h)
+  =p= with_name s f h.
 Proof.
+  intro n.
   case_string s (n_string n); easy.
 Qed.
 
-Lemma iname_eta {A} s (ln : iname A) n :
-  with_name s (project_name s ln) ln n = ln n.
+Lemma iname_eta {A} s (f : iname A) :
+  with_name s (project_name s f) f =p= f.
 Proof.
+  intro n.
   case_string s (n_string n); subst; easy.
 Qed.
 
@@ -605,37 +633,37 @@ Hint Rewrite @iname_beta_project_neq
 
 (* Corollaries of the beta rules *)
 
-Lemma iname_beta_project_drop_eq {A} s n (l : iname A) i :
+Lemma iname_beta_project_drop_eq {A} s n (f : iname A) :
   s = n_string n ->
-  project_name s (drop_name n l) i
-  = drop_idx (n_index n) (project_name (n_string n) l) i.
+  project_name s (drop_name n f)
+  =p= drop_idx (n_index n) (project_name (n_string n) f).
 Proof.
   intro; unfold drop_name; subst.
   autorewrite with rw_names; easy.
 Qed.
 
-Lemma iname_beta_project_drop_neq {A} s n (l : iname A) i :
+Lemma iname_beta_project_drop_neq {A} s n (f : iname A) :
   s <> n_string n ->
-  project_name s (drop_name n l) i
-  = project_name s l i.
+  project_name s (drop_name n f)
+  =p= project_name s f.
 Proof.
   intro; unfold drop_name.
   autorewrite with rw_names; easy.
 Qed.
 
-Lemma iname_beta_project_insert_eq {A} s n a (l : iname A) i :
+Lemma iname_beta_project_insert_eq {A} s n a (f : iname A) :
   s = n_string n ->
-  project_name s (insert_name n a l) i
-  = insert_idx (n_index n) a (project_name (n_string n) l) i.
+  project_name s (insert_name n a f)
+  =p= insert_idx (n_index n) a (project_name (n_string n) f).
 Proof.
   intro; unfold insert_name; subst.
   autorewrite with rw_names; easy.
 Qed.
 
-Lemma iname_beta_project_insert_neq {A} s n a (l : iname A) i :
+Lemma iname_beta_project_insert_neq {A} s n a (f : iname A) :
   s <> n_string n ->
-  project_name s (insert_name n a l) i
-  = project_name s l i.
+  project_name s (insert_name n a f)
+  =p= project_name s f.
 Proof.
   intro; unfold insert_name.
   autorewrite with rw_names; easy.
@@ -645,33 +673,29 @@ Hint Rewrite @iname_beta_project_drop_eq @iname_beta_project_drop_neq
      @iname_beta_project_insert_eq @iname_beta_project_insert_neq
   using (cbn; congruence) : rw_names.
 
-Lemma iname_beta_get {A} n (a : A) l :
-  get_name n (insert_name n a l) = a.
+Lemma iname_beta_get {A} n (a : A) f :
+  get_name n (insert_name n a f) = a.
 Proof.
   autorewrite with rw_names rw_idxs; easy.
 Qed.
 
-Lemma iname_beta_drop {A} n (a : A) l m :
-  drop_name n (insert_name n a l) m = l m.
+Lemma iname_beta_drop {A} n (a : A) f :
+  drop_name n (insert_name n a f) =p= f.
 Proof.
+  intro m.
   case_string (n_string n) (n_string m); try easy.
-  rewrite drop_idx_ext
-    with (l2 := insert_idx (n_index n) a (project_name (n_string n) l))
-    by (intro; autorewrite with rw_names; easy).
   autorewrite with rw_idxs; cbn.
   replace (n_string n) with (n_string m) by easy; easy.
 Qed.
 
-Lemma iname_insert_eta {A} n (l : iname A) m :
-  insert_name n (get_name n l) (drop_name n l) m = l m.
+Lemma iname_insert_eta {A} n (f : iname A) :
+  insert_name n (get_name n f) (drop_name n f) =p= f.
 Proof.
+  intro m.
   case_string (n_string n) (n_string m); try easy.
-  rewrite insert_idx_ext
-    with (l2 := drop_idx (n_index n) (project_name (n_string n) l))
-    by (intro; autorewrite with rw_names; easy).
-  replace (l n)
-    with (get_idx (n_index n) (project_name (n_string n) l)) by easy.
-  autorewrite with rw_idxs.
+  replace (f n)
+    with (get_idx (n_index n) (project_name (n_string n) f)) by easy.
+  autorewrite with rw_idxs; cbn.
   replace (n_string n) with (n_string m); easy.
 Qed.
 
@@ -680,180 +704,76 @@ Hint Rewrite @iname_beta_get @iname_beta_drop @iname_insert_eta
 
 (* Commuting [iname] operations *)
 
-Lemma swap_with_name_with_name {A} s li t lj (ln : iname A) n :
+Lemma swap_with_name_with_name {A} s li t lj (ln : iname A) :
   s <> t ->
-  with_name s li (with_name t lj ln) n
-  = with_name t lj (with_name s li ln) n.
+  with_name s li (with_name t lj ln)
+  =p= with_name t lj (with_name s li ln).
 Proof.
-  intro Hneq.
+  intros Hneq n.
   case_string s (n_string n); try easy.
   case_string t (n_string n); easy.
 Qed.
 
-(* These proofs could really use rewriting under binders ... *)
-
-Lemma swap_drop_name_drop_name {A} n m (l : iname A) o :
-  drop_name n (drop_name m l) o
-  = drop_name (unshift_name n m)
-      (drop_name (shift_name m n) l) o.
+Lemma swap_drop_name_drop_name {A} n m (f : iname A) :
+  drop_name n (drop_name m f)
+  =p= drop_name (unshift_name n m) (drop_name (shift_name m n) f).
 Proof.
+  intro o.
   case_string (n_string n) (n_string m).
   - case_string (n_string m) (n_string o); try easy.
-    rewrite drop_idx_ext
-      with (l2 := drop_idx (n_index m) (project_name (n_string m) l))
-      by (intro; autorewrite with rw_names; easy).
     rewrite swap_drop_idx_drop_idx.
-    apply drop_idx_ext; intro.
-    autorewrite with rw_names; cbn.
     replace (n_string n) with (n_string m) by easy; easy.
   - unfold drop_name.
     rewrite swap_with_name_with_name by easy.
-    apply with_name_ext; intro.
-    + apply drop_idx_ext; intro.
-      autorewrite with rw_names; easy.
-    + apply with_name_ext1; intro.
-      apply drop_idx_ext; intro.
-      autorewrite with rw_names; easy.
+    autorewrite with rw_names; easy.
 Qed.
 
-Lemma swap_insert_name_insert_name {A} n a m b (l : iname A) o :
-  insert_name n a (insert_name m b l) o
-  = insert_name (shift_name n m) b
-      (insert_name (unshift_name m n) a l) o.
+Lemma swap_insert_name_insert_name {A} n a m b (f : iname A) :
+  insert_name n a (insert_name m b f)
+  =p= insert_name (shift_name n m) b
+      (insert_name (unshift_name m n) a f).
 Proof.
+  intro o.
   case_string (n_string n) (n_string m).
   - case_string (n_string m) (n_string o); try easy.
-    rewrite insert_idx_ext
-      with (l2 := insert_idx (n_index m) b (project_name (n_string m) l))
-      by (intro; autorewrite with rw_names; easy).
     rewrite swap_insert_idx_insert_idx.
-    apply insert_idx_ext; intro.
-    autorewrite with rw_names; cbn.
     replace (n_string n) with (n_string m) by easy; easy.
   - unfold insert_name.
     rewrite swap_with_name_with_name by easy.
-    apply with_name_ext; intro.
-    + apply insert_idx_ext; intro.
-      autorewrite with rw_names; easy.
-    + apply with_name_ext1; intro.
-      apply insert_idx_ext; intro.
-      autorewrite with rw_names; easy.
+    autorewrite with rw_names; easy.
 Qed.
 
-Lemma swap_drop_name_insert_name {A} n m a (l : iname A) o :
+Lemma swap_drop_name_insert_name {A} n m a (f : iname A) :
   n <> m ->
-  drop_name n (insert_name m a l) o
-  = insert_name (unshift_name n m) a
-      (drop_name (unshift_name m n) l) o.
+  drop_name n (insert_name m a f)
+  =p= insert_name (unshift_name n m) a
+        (drop_name (unshift_name m n) f).
 Proof.
-  intro Hneq.
+  intros Hneq o.
   case_string (n_string n) (n_string m).
   - case_string (n_string n) (n_string o); try easy.
-    rewrite drop_idx_ext
-      with (l2 := insert_idx (n_index m) a (project_name (n_string m) l))
-      by (intro; autorewrite with rw_names; easy).
-    rewrite swap_drop_idx_insert_idx.
-    + apply insert_idx_ext; intro.
-      autorewrite with rw_names; cbn.
-      replace (n_string n) with (n_string m) by easy.
-      easy.
-    + intro; apply Hneq.
-      replace n with (mkname (n_string n) (n_index n)) by easy.
-      replace (n_string n) with (n_string m) by easy.
-      replace (n_index n) with (n_index m) by easy.
-      easy.
+    rewrite swap_drop_idx_insert_idx
+      by auto using name_neq_string_eq_index_neq.
+    replace (n_string n) with (n_string m) by easy; easy.
   - unfold drop_name, insert_name.
     rewrite swap_with_name_with_name by easy.
-    apply with_name_ext; intro.
-    + apply insert_idx_ext; intro.
-      autorewrite with rw_names; easy.
-    + apply with_name_ext1; intro.
-      apply drop_idx_ext; intro.
-      autorewrite with rw_names; easy.
+    autorewrite with rw_names; easy.
 Qed.
 
-Lemma swap_insert_name_drop_name {A} n m a (l : iname A) o :
-  insert_name n a (drop_name m l) o
-  = drop_name (shift_name n m)
-      (insert_name (shift_name (shift_name n m) n) a l) o.
+Lemma swap_insert_name_drop_name {A} n m a (f : iname A) :
+  insert_name n a (drop_name m f)
+  =p= drop_name (shift_name n m)
+      (insert_name (shift_name (shift_name n m) n) a f).
 Proof.
+  intro o.
   case_string (n_string n) (n_string m).
   - case_string (n_string n) (n_string o); try easy.
-    rewrite insert_idx_ext
-      with (l2 := drop_idx (n_index m) (project_name (n_string m) l))
-      by (intro; autorewrite with rw_names; easy).
     rewrite swap_insert_idx_drop_idx.
-    apply drop_idx_ext; intro.
-    autorewrite with rw_names; cbn.
-    replace (n_string n) with (n_string m) by easy.
-    easy.
+    replace (n_string n) with (n_string m) by easy; easy.
   - unfold drop_name, insert_name.
     rewrite swap_with_name_with_name by easy.
-    apply with_name_ext; intro.
-    + apply drop_idx_ext; intro.
-      autorewrite with rw_names; easy.
-    + apply with_name_ext1; intro.
-      apply insert_idx_ext; intro.
-      autorewrite with rw_names; easy.
-Qed.
-
-(* Pre-composition of [iname name] values *)
-
-Definition compose_name {A} (l1 : iname name) (l2 : iname A) :=
-  fun (n : name) => get_name (get_name n l1) l2.
-
-Lemma compose_name_assoc {A} l1 l2 (l3 : iname A) n :
-  compose_name (compose_name l1 l2) l3 n
-  = compose_name l1 (compose_name l2 l3) n.
-Proof.
-  unfold compose_name; cbn; easy.
-Qed.
-
-Lemma compose_name_id {A} (l : iname A) n :
-  compose_name id_name l n = l n.
-Proof.
-  unfold compose_name; cbn; easy.
-Qed.
-
-Lemma compose_name_drop {A} n l1 (l2 : iname A) m :
-  compose_name (drop_name n l1) l2 m
-  = drop_name n (compose_name l1 l2) m.
-Proof.
-  unfold compose_name.
-  case_string (n_string n) (n_string m); try easy.
-  case_order (n_index n) (n_index m);
     autorewrite with rw_names; easy.
 Qed.
-
-Lemma compose_name_shift {A} n (l : iname A) m :
-  compose_name (shift_name n) l m
-  = drop_name n l m.
-Proof.
-  unfold shift_name; rewrite compose_name_drop.
-  apply drop_name_ext; intro; rewrite compose_name_id; easy.
-Qed.
-
-Lemma compose_name_insert {A} n m l1 (l2 : iname A) o :
-  compose_name (insert_name n m l1) l2 o
-  = insert_name n (get_name m l2) (compose_name l1 l2) o.
-Proof.
-  unfold compose_name.
-  case_string (n_string n) (n_string o); try easy.
-  case_order (n_index n) (n_index o);
-    autorewrite with rw_names; easy.
-Qed.
-
-Lemma compose_name_unshift {A} i (l : iname A) j :
-  compose_name (unshift_name i) l j
-  = insert_name i (get_name i l) l j.
-Proof.
-  unfold unshift_name; rewrite compose_name_insert.
-  apply insert_name_ext; intro; rewrite compose_name_id; easy.
-Qed.
-
-Hint Rewrite @compose_name_assoc @compose_name_id @compose_name_drop
-     @compose_name_shift @compose_name_insert @compose_name_unshift
-  : rw_names.
 
 (* Bound variables are represented by a level *)
 
@@ -868,17 +788,225 @@ Fixpoint level (V : nat) : Set :=
   end.
 Arguments level !V.
 
-(* Functions from [levels]s that we treat like lists *)
-Definition ilevel V A := level V -> A.
+(* Liftable morphisms from [level]s that we treat like streams *)
+Definition ilevel N T M := morph level N T M.
 
-Definition hd_level {V} {A} (l : ilevel (S V) A) := l l0.
+Definition hd_level {N T M} (f : ilevel (S N) T M)
+  : forall V, T (M + V) :=
+  fun V => @f V l0.
 
-Definition tl_level {V} {A} (l : ilevel (S V) A) : ilevel V A :=
-  fun (v : level V) => l (lS v).
+Definition tl_level {N T M} (f : ilevel (S N) T M)
+  : ilevel N T M :=
+  fun V l => f V (lS l).
 
-Definition cons_level {V} {A} a (l : ilevel V A) : ilevel (S V) A :=
-  fun (v : level (S V)) =>
-    match v with
-    | l0 => a
-    | lS v => l v
+Definition cons_level {N} {T : nset} {M}
+  (a : forall V, T (M + V)) (f : ilevel N T M)
+  : ilevel (S N) T M :=
+  fun V l =>
+    match l with
+    | l0 => a V
+    | lS l => f V l
     end.
+
+Arguments hd_level {N T M} f V /.
+Arguments tl_level {N T M} f V l /.
+Arguments cons_level {N T M} a f V !l.
+
+(* Morphism definitions *)
+
+Add Parametric Morphism {N} {T : nset} {M} : (@hd_level N T M)
+    with signature
+      (forall_relation
+         (fun V => pointwise_relation (level (S N + V)) eq)
+         ==>
+         (forall_relation
+            (fun V => @eq (T (M + V)))))
+    as hd_level_mor.
+  intros * Heq; unfold hd_level; intro.
+  rewrite Heq; easy.
+Qed.
+
+Add Parametric Morphism {N} {T : nset} {M} : (@tl_level N T M)
+    with signature
+      (forall_relation
+         (fun V => pointwise_relation (level (S N + V)) eq)
+         ==>
+         (forall_relation
+            (fun V => pointwise_relation (level (N + V)) eq)))
+    as tl_level_mor.
+  intros * Heq; intro; intro; unfold tl_level; cbn.
+  rewrite Heq; easy.
+Qed.
+
+Add Parametric Morphism {N} {T : nset} {M} : (@cons_level N T M)
+    with signature
+      (forall_relation
+         (fun V => @eq (T (M + V)))
+        ==>
+        (forall_relation
+           (fun V => pointwise_relation (level (N + V)) eq)
+           ==>
+           (forall_relation
+              (fun V => pointwise_relation (level (S N + V)) eq))))
+    as cons_level_mor.
+  intros * Heq1 * Heq2; intro a; intro b; unfold cons_level.
+  destruct b; rewrite ?Heq1, ?Heq2; easy.
+Qed.
+
+(* Useful [ilevel level]s *)
+
+Definition id_level {N} : ilevel N level N :=
+  fun V l => l.
+Arguments id_level {N} V l /.
+
+Definition shift_level {N} :=
+  tl_level (@id_level (S N)).
+
+Definition unshift_level N : ilevel (S (S N)) level (S N) :=
+  @cons_level (S N) level (S N) (fun V => l0) (@id_level (S N)).
+
+(* Beta and eta rules for [ilevel] operations *)
+
+Lemma ilevel_beta_hd {N} {T : nset} {M} (a : forall V, T (M + V))
+      (f : ilevel N T M) :
+  hd_level (cons_level a f) = a.
+Proof. easy. Qed.
+
+Lemma ilevel_beta_tl {N} {T : nset} {M} (a : forall V, T (M + V))
+      (f : ilevel N T M) :
+  tl_level (cons_level a f) = f.
+Proof. easy. Qed.
+
+Lemma ilevel_eta {N} {T : nset} {M} (f : ilevel (S N) T M) :
+  cons_level (hd_level f) (tl_level f) =pn= f.
+Proof.
+  intros V l.
+  destruct l; cbn; easy.
+Qed.
+
+Hint Rewrite @ilevel_beta_hd @ilevel_beta_tl @ilevel_eta
+  : rw_levels.
+
+(* Variables are either free names or bound levels *)
+
+Inductive var (V : nat) :=
+| free (n : name)
+| bound (l : level V).
+
+Arguments free {V} n.
+Arguments bound {V} l.
+
+(* Liftable morphisms from [var]s that we treat like pairs *)
+Definition ivar N T M := morph var N T M.
+
+Definition fst_var {N T M} (f : ivar N T M) :
+  forall V, iname (T (M + V)) :=
+    fun V (n : name) => f V (free n).
+
+Definition snd_var {N T M} (f : ivar N T M) : ilevel N T M :=
+    fun V (l : level (N + V)) => f V (bound l).
+
+Definition pair_var {N} {T : nset} {M}
+             (f : forall V, iname (T (M + V)))
+             (g : ilevel N T M) : ivar N T M :=
+  fun V v =>
+    match v with
+    | free n => f V n
+    | bound l => g V l
+    end.
+
+Definition opn_var {N T M} n (f : ivar N T M)
+  : ivar (S N) T M :=
+  pair_var
+    (fun V => drop_name n (fst_var f V))
+    (cons_level (fun V => get_name n (fst_var f V)) (snd_var f)).
+
+Definition cls_var {N T M} n (f : ivar (S N) T M)
+  : ivar N T M :=
+  pair_var
+    (fun V => insert_name n (hd_level (snd_var f) V) (fst_var f V))
+    (tl_level (snd_var f)).
+
+Definition wk_var {N T M} (f : ivar (S N) T M)
+  : ivar N T M :=
+  pair_var (fst_var f) (tl_level (snd_var f)).
+
+Definition bnd_var {N T M} a (f : ivar N T M)
+  : ivar (S N) T M :=
+  pair_var (fst_var f) (cons_level a (snd_var f)).
+
+(* Morphism definitions *)
+
+Add Parametric Morphism {N} {T : nset} {M} : (@hd_level N T M)
+    with signature
+      (forall_relation
+         (fun V => pointwise_relation (level (S N + V)) eq)
+         ==>
+         (forall_relation
+            (fun V => @eq (T (M + V)))))
+    as hd_level_mor.
+  intros * Heq; unfold hd_level; intro.
+  rewrite Heq; easy.
+Qed.
+
+Add Parametric Morphism {N} {T : nset} {M} : (@tl_level N T M)
+    with signature
+      (forall_relation
+         (fun V => pointwise_relation (level (S N + V)) eq)
+         ==>
+         (forall_relation
+            (fun V => pointwise_relation (level (N + V)) eq)))
+    as tl_level_mor.
+  intros * Heq; intro; intro; unfold tl_level; cbn.
+  rewrite Heq; easy.
+Qed.
+
+Add Parametric Morphism {N} {T : nset} {M} : (@cons_level N T M)
+    with signature
+      (forall_relation
+         (fun V => @eq (T (M + V)))
+        ==>
+        (forall_relation
+           (fun V => pointwise_relation (level (N + V)) eq)
+           ==>
+           (forall_relation
+              (fun V => pointwise_relation (level (S N + V)) eq))))
+    as cons_level_mor.
+  intros * Heq1 * Heq2; intro a; intro b; unfold cons_level.
+  destruct b; rewrite ?Heq1, ?Heq2; easy.
+Qed.
+
+(* Useful [ilevel level]s *)
+
+Definition id_level {N} : ilevel N level N :=
+  fun V l => l.
+Arguments id_level {N} V l /.
+
+Definition shift_level {N} :=
+  tl_level (@id_level (S N)).
+
+Definition unshift_level N : ilevel (S (S N)) level (S N) :=
+  @cons_level (S N) level (S N) (fun V => l0) (@id_level (S N)).
+
+(* Beta and eta rules for [ilevel] operations *)
+
+Lemma ilevel_beta_hd {N} {T : nset} {M} (a : forall V, T (M + V))
+      (f : ilevel N T M) :
+  hd_level (cons_level a f) = a.
+Proof. easy. Qed.
+
+Lemma ilevel_beta_tl {N} {T : nset} {M} (a : forall V, T (M + V))
+      (f : ilevel N T M) :
+  tl_level (cons_level a f) = f.
+Proof. easy. Qed.
+
+Lemma ilevel_eta {N} {T : nset} {M} (f : ilevel (S N) T M) :
+  cons_level (hd_level f) (tl_level f) =pn= f.
+Proof.
+  intros V l.
+  destruct l; cbn; easy.
+Qed.
+
+Hint Rewrite @ilevel_beta_hd @ilevel_beta_tl @ilevel_eta
+  : rw_levels.
+
